Micro_C_Examples/C_Struct_Examples.thy
@@ -1,0 +1,74 @@
+(* Copyright Amazon.com, Inc. or its affiliates. All Rights Reserved.
+   SPDX-License-Identifier: MIT *)
+
+theory C_Struct_Examples
+  imports
+    "Micro_C_Parsing_Frontend.C_To_Core_Translation"
+    "Shallow_Micro_C.C_Arithmetic_Rules"
+    "Micro_Rust_Std_Lib.StdLib_All"
+begin
+
+micro_rust_record c_point
+
+section \<open>C Struct Verification\<close>
+
+text \<open>
+  This theory demonstrates verification of C code operating on structs.
+  The function @{text swap_coords} swaps the x and y fields of a
+  point struct via a pointer.
+\<close>
+
+locale c_struct_verification_ctx =
+    reference reference_types +
+    ref_c_int: reference_allocatable reference_types _ _ _ _ _ _ _ c_int_prism +
+    ref_c_point: reference_allocatable reference_types _ _ _ _ _ _ _ c_point_prism
+  for
+    reference_types :: \<open>'s::{sepalg} \<Rightarrow> 'addr \<Rightarrow> 'gv \<Rightarrow> 'abort \<Rightarrow> 'i prompt \<Rightarrow> 'o prompt_output \<Rightarrow> unit\<close>
+    and c_int_prism :: \<open>('gv, c_int) prism\<close>
+    and c_point_prism :: \<open>('gv, c_point) prism\<close>
+begin
+
+adhoc_overloading store_reference_const \<rightleftharpoons> ref_c_int.new
+adhoc_overloading store_reference_const \<rightleftharpoons> ref_c_point.new
+adhoc_overloading store_update_const \<rightleftharpoons> update_fun
+
+micro_c_translate \<open>
+struct point {
+  int x;
+  int y;
+};
+void swap_coords(struct point *p) {
+  int t = p->x;
+  p->x = p->y;
+  p->y = t;
+}
+\<close>
+
+thm c_swap_coords_def
+
+text \<open>
+  The contract for swap\_coords: given a reference to a c\_point with value
+  @{text pval}, after execution the x and y fields are swapped.
+\<close>
+definition c_swap_coords_contract ::
+    \<open>('addr, 'gv, c_point) Global_Store.ref \<Rightarrow>
+     'gv \<Rightarrow> c_point \<Rightarrow> ('s, 'a, 'b) function_contract\<close> where
+  \<open>c_swap_coords_contract pref pg pval \<equiv>
+    let pre  = can_alloc_reference \<star>
+               pref \<mapsto>\<langle>\<top>\<rangle> pg\<down>pval in
+    let post = \<lambda> _.
+               can_alloc_reference \<star>
+               pref \<mapsto>\<langle>\<top>\<rangle> (\<lambda>_. make_c_point (c_point_y pval) (c_point_x pval)) \<sqdot> (pg\<down>pval) in
+    make_function_contract pre post\<close>
+ucincl_auto c_swap_coords_contract
+
+lemma c_swap_coords_spec:
+  shows \<open>\<Gamma>; c_swap_coords pref \<Turnstile>\<^sub>F c_swap_coords_contract pref pg pval\<close>
+  apply (crush_boot f: c_swap_coords_def contract: c_swap_coords_contract_def)
+  apply crush_base
+  apply (all \<open>cases pval; simp add: c_point_c_point_x_update_explicit c_point_c_point_y_update_explicit\<close>)
+  done
+
+end
+
+end
