Micro_C_Examples/Micro_C_Examples.thy
@@ -4,6 +4,8 @@
 theory Micro_C_Examples
   imports
     Simple_C_Functions
+    C_Struct_Examples
+    C_Array_Examples
     "Micro_C_Interfaces.Micro_C_Interfaces"
 begin
 end
